Generalise contract transfer theorem  (#4)
* Add more general definition of simulation (simulated_termination_def)
* Add refinement theorems (simulated_simulated_termination and simulated_fail_simulated_termination)
* Generalise contract refinement theorem, multistep simulation and refinement theorem and contract transfer theorem

examples/ijr/contractTransferScript.sml
@@ -5,10 +5,38 @@ open listTheory;
 open bir_programTheory bir_htTheory bir_program_multistep_propsTheory;
 open HolBACoreSimps;
 
-open resolutionTheory simulationTheory;
+open resolutionTheory simulationTheory simulationFailTheory;
 
 val _ = new_theory "contractTransfer";
 
+
+Definition simulated_termination_def:
+  simulated_termination (p: 'a bir_program_t) (p': 'a bir_program_t) =
+  ∀s l s' o2 m2 n2.
+    s.bst_pc = bir_block_pc l ⇒
+    MEM l (bir_labels_of_program p) ⇒
+
+    exec_to_prog p' s p = BER_Ended o2 m2 n2 s' ⇒
+    ~(bir_state_is_terminated s') ⇒
+    (∃o1 m1 n1.
+      exec_to_prog p s p = BER_Ended o1 m1 n1 s')
+End
+
+Theorem simulated_simulated_termination:
+  ∀p p'. simulated p p' ⇒ simulated_termination p p'
+Proof
+FULL_SIMP_TAC (std_ss++holBACore_ss)
+              [simulated_def, simulated_termination_def,
+               bir_state_is_terminated_def]
+QED
+
+Theorem simulated_fail_simulated_termination:
+  ∀p p'. simulated_fail p p' ⇒ simulated_termination p p'
+Proof
+FULL_SIMP_TAC (std_ss++holBACore_ss)
+              [simulated_fail_def, simulated_termination_def,
+               bir_state_is_terminated_def]
+QED
 
 Definition exec_to_prog_n_def:
   exec_to_prog_n p s pls n =
@@ -16,23 +44,23 @@ Definition exec_to_prog_n_def:
 End
 
 (*TODO: Strenthen simulation definitions wrt observations and steps?*)
-Definition simulated_n_def:
-  simulated_n p p' =
+Definition simulated_termination_n_def:
+  simulated_termination_n p p' =
   ∀n s l s' os2 m2 n2.
     s.bst_pc = bir_block_pc l ⇒
     MEM l (bir_labels_of_program p) ⇒
 
     exec_to_prog_n p' s p n = BER_Ended os2 m2 n2 s' ⇒
-    ~(∃l'. s'.bst_status = BST_JumpOutside l') ⇒
+    ~(bir_state_is_terminated s') ⇒
     (∃os1 m1 n1.
       exec_to_prog_n p s p n = BER_Ended os1 m1 n1 s')
 End
 
-Theorem simulated_simulated_n:
-  ∀p p'. simulated p p' ⇒ simulated_n p p'
+Theorem simulated_termination_simulated_termination_n:
+  ∀p p'. simulated_termination p p' ⇒ simulated_termination_n p p'
 Proof
 REPEAT STRIP_TAC >>
-SIMP_TAC std_ss [simulated_n_def, exec_to_prog_n_def] >>
+SIMP_TAC std_ss [simulated_termination_n_def, exec_to_prog_n_def] >>
 Q.ABBREV_TAC ‘ls = bir_labels_of_program p’ >>
 
 Induct_on ‘n’ >- (
@@ -48,22 +76,16 @@ SIMP_TAC (std_ss++holBACore_ss) [] >>
 rename1 ‘_ = BER_Ended os21 m21 n21 s2’ >>
 
 (*There is a contradiction or p takes the same step*)
-Cases_on ‘(∃l'. s2.bst_status = BST_JumpOutside l')’ >- (
+Cases_on ‘bir_state_is_terminated s2’ >- (
   FULL_SIMP_TAC (list_ss++holBACore_ss) [bir_state_is_terminated_def,
                                          bir_exec_to_labels_n_REWR_TERMINATED] >>
   STRIP_TAC >> FULL_SIMP_TAC (std_ss++holBACore_ss) []
 ) >>
 subgoal ‘(∃os11 m11 n11.
             bir_exec_to_labels (set ls) p s = BER_Ended os11 m11 n11 s2)’ >- (
-  FULL_SIMP_TAC (std_ss++holBACore_ss) [simulated_def, exec_to_prog_def]
+  FULL_SIMP_TAC (std_ss++holBACore_ss) [simulated_termination_def, exec_to_prog_def]
 ) >>
 ASM_SIMP_TAC (std_ss++holBACore_ss) [] >>
-
-(*If programs are terminated, rest of steps are same (needed to use induction hypothesis)*)
-Cases_on ‘(bir_state_is_terminated s2)’ >- (
-  FULL_SIMP_TAC (list_ss++holBACore_ss) [bir_state_is_terminated_def,
-                                         bir_exec_to_labels_n_REWR_TERMINATED]
-) >>
 
 (*Program p' takes the rest of the steps*)
 Cases_on ‘bir_exec_to_labels_n (set ls) p' s2 n’ >>
@@ -129,8 +151,8 @@ Definition simulated_contract_def:
       bir_exec_to_labels ls p s = BER_Ended os1 m1 n1 s')
 End
 
-Theorem simulated_simulated_contract:
-  ∀p p'. simulated p p' ⇒ simulated_contract p p'
+Theorem simulated_termination_simulated_contract:
+  ∀p p'. simulated_termination p p' ⇒ simulated_contract p p'
 Proof
 REPEAT STRIP_TAC >>
 SIMP_TAC std_ss [simulated_contract_def, exec_to_prog_n_def] >>
@@ -146,10 +168,8 @@ rename1 ‘_ = BER_Ended _ _ n2' _’ >>
 (*Use simulation hypothesis*)
 subgoal ‘∃os1 m1 n1. bir_exec_to_labels_n (set pls) p s n =
                      BER_Ended os1 m1 n1 s'’ >- (
-  subgoal ‘~(∃l'. s'.bst_status = BST_JumpOutside l')’ >- (
-    FULL_SIMP_TAC (std_ss++holBACore_ss) [bir_state_is_terminated_def]
-  ) >>
-  METIS_TAC [simulated_simulated_n, simulated_n_def, exec_to_prog_n_def]
+  METIS_TAC [simulated_termination_simulated_termination_n,
+             simulated_termination_n_def, exec_to_prog_n_def]
 ) >>
 
 (*Restrict label set*)
@@ -165,15 +185,15 @@ subgoal ‘∃n1'.bir_exec_to_labels ls p s = BER_Ended os1 m1 n1' s'’ >- (
     Q.PAT_X_ASSUM ‘∀n'. _’ (fn thm => ASSUME_TAC (Q.SPEC ‘n'’ thm)) >>
     REV_FULL_SIMP_TAC std_ss [] >>
 
-    subgoal ‘~(∃l'. s''.bst_status = BST_JumpOutside l')’ >- (
+    subgoal ‘~bir_state_is_terminated s''’ >- (
       FULL_SIMP_TAC std_ss [bir_exec_to_labels_n_def] >>
-      ‘~bir_state_is_terminated s''’ by
-        IMP_RES_TAC bir_exec_steps_GEN_decrease_max_steps_Ended_terminated >>
-      FULL_SIMP_TAC (std_ss++holBACore_ss) [bir_state_is_terminated_def]
+      IMP_RES_TAC bir_exec_steps_GEN_decrease_max_steps_Ended_terminated
     ) >>
+
     subgoal ‘∃os' c1' c2''. bir_exec_to_labels_n (set pls) p s n' =
                             BER_Ended os' c1' c2'' s''’ >- (
-      METIS_TAC [simulated_simulated_n, simulated_n_def, exec_to_prog_n_def]
+      METIS_TAC [simulated_termination_simulated_termination_n,
+                 simulated_termination_n_def, exec_to_prog_n_def]
     ) >>
 
     PROVE_TAC []
@@ -186,7 +206,7 @@ QED
 
 Theorem contract_transfer:
   ∀ p p' l ls pre post.
-    simulated p p' ⇒
+    simulated_termination p p' ⇒
     bir_vars_of_program p' = bir_vars_of_program p ⇒
 
     MEM l (bir_labels_of_program p) ⇒
@@ -198,9 +218,8 @@ Proof
 SIMP_TAC std_ss [bir_exec_to_labels_triple_def] >>
 REPEAT STRIP_TAC >>
 
-Q.PAT_X_ASSUM ‘simulated p p'’
-  (fn thm => ASSUME_TAC (MATCH_MP simulated_simulated_contract thm)) >>
-
+Q.PAT_X_ASSUM ‘simulated_termination p p'’
+  (fn thm => ASSUME_TAC (MATCH_MP simulated_termination_simulated_contract thm)) >>
 Q.PAT_X_ASSUM ‘∀s'. _’ (fn thm => ASSUME_TAC (Q.SPEC ‘s’ thm)) >>
 REV_FULL_SIMP_TAC std_ss [] >>
 rename1 ‘_ = BER_Ended o2 m2 n2 s'’ >>
@@ -219,10 +238,11 @@ subgoal ‘∃s1 o1 m1 n1. bir_exec_to_labels ls p s =
 PROVE_TAC []
 QED
 
-(*Sanity check*)
+(*Sanity checks*)
+
 Theorem resolved_contract_transfer:
   ∀l1 v sl p p' l ls pre post.
-    resolved l1 v sl p p' ⇒
+    resolved l1 v sl p p'  ⇒
     bir_vars_of_program p' = bir_vars_of_program p ⇒
 
     MEM l (bir_labels_of_program p) ⇒
@@ -231,8 +251,27 @@ Theorem resolved_contract_transfer:
     bir_exec_to_labels_triple p' l ls pre post ⇒
     bir_exec_to_labels_triple p l ls pre post
 Proof
-PROVE_TAC [contract_transfer, resolved_simulated]
+PROVE_TAC [resolved_simulated,
+           contract_transfer,
+           simulated_simulated_termination]
+QED
+
+Theorem resolved_fail_contract_transfer:
+  ∀l1 v p p' l ls pre post.
+    resolved_fail l1 v p p' ⇒
+    bir_vars_of_program p' = bir_vars_of_program p ⇒
+
+    MEM l (bir_labels_of_program p) ⇒
+    ls SUBSET (set (bir_labels_of_program p)) ⇒
+
+    bir_exec_to_labels_triple p' l ls pre post ⇒
+    bir_exec_to_labels_triple p l ls pre post
+Proof
+PROVE_TAC [resolved_fail_simulated_fail,
+           simulated_fail_simulated_termination,
+           contract_transfer]
 QED
 
 
 val _ = export_theory();
+
